src/Bridges.v
@@ -1,0 +1,3 @@
+(* Bridges for different Inductive Definition. 
+    Can be seen as a wrapper as a Main prgoram
+*)
